Cm/Eval5.lean
@@ -1,0 +1,212 @@
+import Mathlib.Data.Nat.Notation
+
+/-
+Automatic currying is quite nice, but I think we could
+make it more obvious when it's required.
+
+π could do this.
+Can derive next from π.
+
+π is like the opposite of both.
+
+π x_case xs_case
+
+π fn nil matches a list with only one thing in it.
+
+The other issue is control flow.
+Both handles one direction,
+but what about the other?
+
+We need a better way to achieve nesting.
+
+With π, we replace read with id.
+
+Append is fine.
+
+An advantage with removing read and next is
+that we no longer have to worry about pipelining.
+
+Can we clean up both? Currently, π will just fail
+if we don't have enough arguments.
+
+I see no reason why we can't have an uncurried
+and curried layer.
+
+Since we have pattern matching now,
+what do we do with the extra arguments?
+Just get rid of them.
+
+Idea:
+- we denote values with no arguments as (:: val nil)
+
+Another idea:
+- both will only combine (:: _ nil) functions
+with arbitrary parameters.
+
+Currying will handle more than that.
+-/
+
+open Std (Format)
+open Std (ToFormat)
+
+inductive Expr where
+  | cons   : Expr
+    → Expr
+    → Expr
+  | π      : Expr
+    → Expr
+    → Expr
+  | id     : Expr
+  | const  : Expr
+  | both   : Expr
+    → Expr
+    → Expr
+  | nil    : Expr
+  | symbol : String
+    → Expr
+deriving Repr, BEq
+
+open Expr
+
+def Expr.fmt (e : Expr) : Format :=
+  match e with
+  | .π a b => .paren <| "π " ++ a.fmt ++ .line ++ b.fmt
+  | .cons (.cons a b) (.cons c d) =>
+    ":: " ++ (.group <| .nest 2 <| (.paren (Expr.cons a b).fmt) ++ Format.line ++ (.paren (Expr.cons c d).fmt))
+  | .cons (.cons a b) xs =>
+    ":: " ++ (.group <| .nest 2 <| (.paren (Expr.cons a b).fmt) ++ Format.line ++ xs.fmt)
+  | .cons x (.cons a b) =>
+    ":: " ++ (.group <| .nest 2 <| x.fmt ++ Format.line ++ (.paren (Expr.cons a b).fmt))
+  | .cons x xs =>
+    ":: " ++ (.group <| .nest 2 <| x.fmt ++ Format.line ++ xs.fmt)
+  | id => "id"
+  | .const => "const"
+  | .both f g => .paren ("both " ++ (.group <| .nest 2 <| (.paren f.fmt) ++ Format.line ++ (.paren g.fmt)))
+  | .nil => "nil"
+  | symbol s => .paren ("symbol " ++ ("\"" ++ s ++ "\""))
+
+instance Expr.instToFormat : ToFormat Expr where
+  format := Expr.fmt
+
+instance Expr.instToString : ToString Expr where
+  toString := toString ∘ Expr.fmt
+
+notation "::" => Expr.cons
+
+def Expr.push_back (val : Expr) : Expr → Option Expr
+  | :: x nil => do pure <| :: x val
+  | :: x xs => do pure <| :: x (← push_back val xs)
+  | _ => .none
+
+def mk_app (f x : Expr) : Option Expr :=
+  Expr.push_back (:: x nil) f
+
+def mk_app' (f : Option Expr) (x : Expr) : Option Expr := do
+  Expr.push_back (:: x nil) (← f)
+
+notation "f*" => mk_app'
+notation "f$" => mk_app
+
+example : Expr.push_back (:: (symbol "zero") nil) (:: (symbol "succ") nil) =
+  (:: (symbol "succ") (:: (symbol "zero") nil)) := rfl
+
+def step_uncurry (e : Expr) (with_logs : Bool := false) : Option Expr := do
+  if with_logs then
+    dbg_trace e
+
+  match e with
+  | :: .id x => pure x
+  | :: (π a nil) (:: x nil) => do
+    let a' ← step_uncurry (:: a x)
+    pure <| :: a' nil
+  | :: (π a b) (:: x xs) => do
+    let a' ← step_uncurry (:: a x)
+    let b' ← step_uncurry (:: b xs)
+    pure <| :: a' b'
+  | :: (:: const x) _ => pure x
+  | :: (both f g) l =>
+    let g' ← step_uncurry (:: g l)
+    match (← step_uncurry (:: f l)) with
+    | :: v nil =>
+      pure <| :: v (:: g' nil)
+    | _ => .none
+  | :: f x => :: (← step_uncurry f) x
+  | _ => .none
+
+def try_step_n (f : Expr → Option Expr) (n : ℕ) (e : Expr) (with_logs : Bool := false) : Option Expr := do
+  if n = 0 then
+    pure e
+  else
+    let e' ← f e
+    (try_step_n f (n - 1) e' with_logs) <|> (pure e')
+
+def do_step (f : Expr → Option Expr) (e : Expr) (with_logs : Bool := false):= try_step_n f 20 e with_logs
+
+namespace church'
+
+/-
+zero f x = x
+
+Note: may considering changing the right branch
+to keep x's arguments floating around?
+Other branch would be
+(:: zero (:: f (:: x (:: other
+we can discard those.
+-/
+def zero : Expr :=
+  π (:: const id) (π id nil)
+
+/-
+n(f, x)
+-/
+def succ.nfx : Expr :=
+  π id (π id (π id nil))
+
+/-
+Selects f out of succ(n, f, x) as
+(:: f nil)
+-/
+def succ.f : Expr :=
+  π (:: const id) (π id nil)
+
+def succ : Expr :=
+  both (
+
+#eval do_step step_uncurry (:: zero (:: (symbol "f") (:: (symbol "x") nil)))
+
+def succ.n : Expr := read
+
+def succ.f : Expr :=
+  (:: next read)
+
+def succ.x : Expr :=
+  (:: next (:: next read))
+
+def succ.fx : Expr :=
+  (both succ.f (both succ.x nil))
+
+def succ.nfx : Expr :=
+  (both succ.n succ.fx)
+
+def succ.f_append : Expr :=
+  (both (:: const append) (both succ.f nil))
+
+def succ : Expr :=
+  both succ.f_append (both succ.nfx nil)
+
+def succ' : Expr :=
+  both (both (:: const append) (both (:: const (symbol ("f"))) (:: const nil))) (:: const (symbol "nfx"))
+
+-- nfx outputs the correct value
+#eval do_step step (:: succ.nfx (:: zero (:: (symbol "f") (:: (symbol "x") nil)))) == some (symbol "x")
+
+-- succ outputs the correct value
+-- succ 0 f x = :: f (:: (0 f x) nil)
+-- we should assume this is a single argument
+#eval do_step step (:: succ (:: zero (:: (symbol "f") (:: (symbol "x") nil)))) == some (:: (symbol "f") (:: (symbol "x") nil))
+
+-- curried form
+#eval do_step step (:: succ.nfx (:: zero nil))
+#eval ToFormat.format <$> do_step step (:: (:: succ.nfx (:: zero nil)) (:: (symbol "f") (:: (symbol "x") nil)))
+
+end church'
